<?xml version="1.0" encoding="UTF-8"?>
<!--
 copyright (c) 2015, Gabriel A. Weaver, Information Trust Institute
   at the University of Illinois, Urbana-Champaign.

  This file is part of the Cyber-Physical Topology Language for
    the Power domain.

  This ontology is available under the Creative Commons 
  Attribution-ShareAlike License.  Details about this license
  are available at the following URL:

  http://creativecommons.org/licenses/by-sa/3.0/legalcode 
 -->
<rdf:RDF
    xmlns:dc="http://purl.org/dc/elements/1.1/"
    xmlns:owl="http://www.w3.org/2002/07/owl#"
    xmlns:rdf="http://www.w3.org/1999/02/22-rdf-syntax-ns#"
    xmlns:rdfs="http://www.w3.org/2000/01/rdf-schema#"
    xmlns:snet="http://cptl-c.org/power/2015/07/substation_network/"
    xmlns:syard="http://cptl-c.org/power/2015/07/substation_yard/">
  
  <owl:Ontology rdf:about="http://cptl-c.org/power/2015/07/substation_network">
    <dc:title>Substation Network</dc:title>
    <dc:description>An ontology to describe components of a substation 
      network.</dc:description>
  </owl:Ontology>

  <owl:Class rdf:about="http://cptl-c.org/power/2015/07/substation_network/RTU">
    <rdfs:subClassOf rdf:resource="http://cptl-c.org/core/2014/07/core/Asset"/>
    <rdfs:label xml:lang="en">RTU</rdfs:label>
    <rdfs:comment>A remote terminal unit (RTU) is a
    microprocessor-controlled electronic device that interfaces
    objects in the physical world to a SCADA ssytem by transmitting
    telemetry data to a master
    system. (http://en.wikipedia.org/wiki/Remote_Terminal_Unit)</rdfs:comment>
  </owl:Class>

  <owl:Class rdf:about="http://cptl-c.org/power/2015/07/substation_network/Switch">
    <rdfs:subClassOf rdf:resource="http://cptl-c.org/enterprise/2015/07/enterprise_network/Switch"/>
    <rdfs:label xml:lang="en">Switch</rdfs:label>
    <rdfs:comment>A network switch (also called switching hub,
    bridging hub, officially MAC bridge[1]) is a computer networking
    device that connects devices together on a computer network, by
    using packet switching to receive, process and forward data to the
    destination device. Unlike less advanced network hubs, a network
    switch forwards data only to one or multiple devices that need to
    receive it, rather than broadcasting the same data out of each of
    its ports. (http://en.wikipedia.org/wiki/Network_switch)</rdfs:comment>
  </owl:Class>

  <!-- Relays -->
  <owl:Class rdf:about="http://cptl-c.org/power/2015/07/substation_network/Relay">
    <rdfs:subClassOf rdf:resource="http://cptl-c.org/core/2014/07/core/Asset"/>
    <rdfs:label xml:lang="en">Relay</rdfs:label>
    <rdfs:comment>A device designed to trip a circuit breaker when a fault
    is detected. (http://en.wikipedia.org/wiki/Protective_relay)</rdfs:comment>
  </owl:Class>

  <owl:Class rdf:about="http://cptl-c.org/power/2015/07/substation_network/DistanceRelay">
    <rdfs:subClassOf rdf:resource="snet:Relay"/>
    <rdfs:label xml:lang="en">Distance Relay</rdfs:label>
    <rdfs:comment>The most common form of protection on high voltage transmission
    systems is distance relay protection.  Power lines have set impedance per kilometre and using 
    this value and comparing voltage and current the distance to a fault can be determined. 
    (http://en.wikipedia.org/wiki/Protective_relay#Distance_relay)</rdfs:comment>
  </owl:Class>

  <owl:Class rdf:about="http://cptl-c.org/power/2015/07/substation_network/OvercurrentRelay">
    <rdfs:subClassOf rdf:resource="snet:Relay"/>
    <rdfs:label xml:lang="en">Overcurrent Relay</rdfs:label>
    <rdfs:comment>A digital over current relay is a protective relay
    which operates when the load current exceeds a pickup value
    (http://en.wikipedia.org/wiki/Protective_relay#Over_current_relay)</rdfs:comment>
  </owl:Class>

  <owl:Class rdf:about="http://cptl-c.org/power/2015/07/substation_network/ReversePowerRelay">
    <rdfs:subClassOf rdf:resource="snet:Relay"/>
    <rdfs:label xml:lang="en">Reverse Power Relay</rdfs:label>
    <rdfs:comment> A reverse power relay is a directional power relay
    that is used to monitor the power from a generator running in
    parallel with another generator or the utility. The function of
    the reverse power relay is to prevent a reverse power condition in
    which power flows from the bus bar into the generator. This
    condition can occur when there is a failure in the prime mover
    such as an engine or a turbine which drives the
    generator. (http://www.electrotechnik.net/2009/06/reverse-power-relay-function-and.html)</rdfs:comment>
  </owl:Class>
  
  <!-- Relations -->
  <owl:ObjectProperty rdf:about="http://cptl-c.org/power/2015/07/substation_network/hasBreakerConnections">
    <rdfs:subClassOf rdf:resource="http://cptl-c.org/core/2014/07/core/hasLink"/>
    <rdfs:label xml:lang="en">Has Breaker Connections</rdfs:label>
        <rdfs:comment>Connections from a relay to a breaker consist of (1) high-side voltage (2) low-side voltage,
        (3) a current loop, (4) breaker status, and (5) a breaker control line.</rdfs:comment>
	<rdfs:domain rdf:resource="snet:Relay"/>
	<rdfs:range rdf:resource="syard:Breaker"/>
  </owl:ObjectProperty>

</rdf:RDF>
