<?xml version="1.0" encoding="UTF-8"?>
<!--
 copyright (c) 2015, Gabriel A. Weaver, Information Trust Institute
   at the University of Illinois, Urbana-Champaign.

  This file is part of the Cyber-Physical Topology Language for
    the Power domain.

  This ontology is available under the Creative Commons 
  Attribution-ShareAlike License.  Details about this license
  are available at the following URL:

  http://creativecommons.org/licenses/by-sa/3.0/legalcode 
  -->

<!DOCTYPE rdf:RDF [
    <!ENTITY foaf "http://xmlns.com/foaf/0.1/" >
    <!ENTITY owl "http://www.w3.org/2002/07/owl#" >
    <!ENTITY dc "http://purl.org/dc/elements/1.1/" >
    <!ENTITY xsd "http://www.w3.org/2001/XMLSchema#" >
    <!ENTITY devos "http://cptl-c.org/device/2014/07/os/" >
    <!ENTITY devfs "http://cptl-c.org/device/2015/05/fs/" >
    <!ENTITY rdfs "http://www.w3.org/2000/01/rdf-schema#" >
    <!ENTITY rdf "http://www.w3.org/1999/02/22-rdf-syntax-ns#" >
]>

<rdf:RDF
    xmlns:dc="http://purl.org/dc/elements/1.1/"
    xmlns:foaf="http://xmlns.com/foaf/0.1/"
    xmlns:owl="http://www.w3.org/2002/07/owl#"
    xmlns:rdf="http://www.w3.org/1999/02/22-rdf-syntax-ns#"
    xmlns:rdfs="http://www.w3.org/2000/01/rdf-schema#"
    xmlns:devos="http://cptl-c.org/device/2014/07/os/"
    xmlns:devfs="http://cptl-c.org/device/2015/05/fs/"> 

  <owl:Ontology rdf:about="http://cptl-c.org/device/2015/05/fs">
    <dc:title>A rudimentary ontology for filesystem hierarchies and permissions </dc:title>
    <dc:description>OS-level data structures to describe systems.</dc:description>
  </owl:Ontology>


  <owl:Class rdf:about="http://cptl-c.org/device/2015/05/fs/File">
    <rdfs:label xml:lang="en">File</rdfs:label>
    <rdfs:comment>A computer file is a resource for storing
    information, which is available to a computer program and is
    usually based on some kind of durable storage. A file is "durable"
    in the sense that it remains available for other programs to use
    after the program that created it has finished executing. Computer
    files can be considered as the modern counterpart of paper
    documents which traditionally are kept in office and library
    files, and this is the source of the
    term. (http://en.wikipedia.org/wiki/Computer_file)</rdfs:comment>
  </owl:Class>

  <owl:Class rdf:about="http://cptl-c.org/device/2015/05/fs/FilePath">
    <rdfs:subClassOf rdf:resource="http://cptl-c.org/core/2014/07/core/Path"/>
    <rdfs:label xml:lang="en">File Path</rdfs:label>
    <rdfs:comment>A path, the general form of the name of a file or
    directory, specifies a unique location in a file system. A path
    points to a file system location by following the directory tree
    hierarchy expressed in a string of characters in which path
    components, separated by a delimiting character, represent each
    directory. (http://en.wikipedia.org/wiki/Path_(computing))</rdfs:comment>
  </owl:Class>
  
  <owl:Class rdf:about="http://cptl-c.org/device/2015/05/fs/Directory">
    <rdfs:subClassOf rdf:resource="http://cptl-c.org/device/2015/05/fs/File"/>
    <rdfs:label xml:lang="en">Directory</rdfs:label>
    <rdfs:comment>In computing, a directory is a file system
    cataloging structure which contains references to other computer
    files, and possibly other
    directories. (http://en.wikipedia.org/wiki/Directory_(computing))</rdfs:comment>
  </owl:Class>

  <owl:ObjectProperty rdf:about="http://cptl-c.org/device/2015/05/fs/inDirectory">
    <rdfs:label xml:lang="en">In Directory</rdfs:label>
    <rdfs:comment>Denotes that a file is contained within a directory.</rdfs:comment>
    <rdfs:domain rdf:resource="&devfs;File"/>
    <rdfs:range rdf:resource="&devfs;Directory"/>
  </owl:ObjectProperty>

  <owl:ObjectProperty rdf:about="http://cptl-c.org/device/2015/05/fs/hasLinkTo">
    <rdfs:label xml:lang="en">Has Link To</rdfs:label>
    <rdfs:comment>Denotes that a file path resolves to another file path via a symlink, alias, or shortcut.</rdfs:comment>
    <rdfs:domain rdf:resource="&devfs;FilePath"/>
    <rdfs:range rdf:resource="&devfs;FilePath"/>
  </owl:ObjectProperty>

  <owl:ObjectProperty rdf:about="http://cptl-c.org/device/2015/05/fs/canRead">
    <rdfs:label xml:lang="en">Can Read</rdfs:label>
    <rdfs:comment>Denotes that a user account has permission to read from a
    file.  Currently, we use the FOAF ontology to denote a user account, although
    these accounts may be local to a machine, not online.</rdfs:comment>
    <rdfs:domain rdf:resource="&foaf;OnlineAccount"/>
    <rdfs:range rdf:resource="&devfs;File"/>
  </owl:ObjectProperty>

  <owl:ObjectProperty rdf:about="http://cptl-c.org/device/2015/05/fs/canWrite">
    <rdfs:label xml:lang="en">Can Write</rdfs:label>
    <rdfs:comment>Denotes that a user account has permission to write
    to a file.  Currently, we use the FOAF ontology to denote a user
    account, although these accounts may be local to a machine, not
    online.</rdfs:comment>
    <rdfs:domain rdf:resource="&foaf;OnlineAccount"/>
    <rdfs:range rdf:resource="&devfs;File"/>
  </owl:ObjectProperty>

  <owl:ObjectProperty rdf:about="http://cptl-c.org/device/2015/05/fs/canRead">
    <rdfs:label xml:lang="en">Can Read</rdfs:label>
    <rdfs:comment>Denotes that a user account has permission to execute a 
    file.  Currently, we use the FOAF ontology to denote a user account, although
    these accounts may be local to a machine, not online.</rdfs:comment>
    <rdfs:domain rdf:resource="&foaf;OnlineAccount"/>
    <rdfs:range rdf:resource="&devfs;File"/>
  </owl:ObjectProperty>
  
</rdf:RDF>
